---
aliases: 
tags: 
creation date: Wednesday, August 10th 2022, 12:23 pm
date updated: Wednesday, August 10th 2022, 12:28 pm
---
![[Pasted image 20220810122438.png]]

Factoring gets us $\frac{(x+4)(x-3)}{(x+3)(x-3)} = \frac{x+4}{x+3} \to 7/6$

![[Pasted image 20220810122553.png]]

Factoring again:
$$ \frac{2(x-2)(x-2)}{(x+5)(x-2)} = \frac{2(x-2)}{(x+5)}$$
so our limits are $0$ and $2$.

3) let $y = e^x$ then we have $\frac{1/y + 2y}{2/y + y}$ which straightforwardly becomes $\frac{2y^2 + 1}{y^2 + 2}$. As $x \to \infty, y \to \infty$; as $x \to -\infty$, $y \to0$. The positive limit is clear - 2. The negative limit is 1/2

![[Pasted image 20220810123645.png]]

a) 1/2
b)
$$\frac{(\sqrt{x^2 + x} - x)((\sqrt{x^2 + x} + x)}{(\sqrt{x^2 + x} + x)}$$
$$\frac{x^2 + x-x^2}{\sqrt{x^2 + x} + x}$$
so the top is roughly order $x and the bottom $2x$. That gives us 1/2?

