---
date updated: 2022-03-11 16:37

notetype: "Math Class Note"
cssclass: math-class-note

tags: 
- '#classnotes'
- '#ğŸš§'
---

# [[18.06 Practice 1]]
Part of [[@Review of Linear Algebra Index]]

### Test Probs 1

Problem 2.1: In the two-by-two system of linear equations below, what  
multiple of the first equation should be subtracted from the second equaÂ­  
tion when using the method of elimination? Convert this system of equaÂ­  
tions to matrix form, apply elimination (what are the pivots?), and use  
back substitution to find a solution. Try to check your work before lookÂ­  
ing up the answer.  
2x + 3y = 5  
6x + 15y = 12  

part 1: 3
part 2:

$$\begin{matrix}
2 & 3 &| & 5 \\
6 & 15 & | & 12
\end{matrix}$$

$$\begin{matrix}
2 & 3 &| & 5 \\
0 & 6 & | & -3
\end{matrix}$$

So $6 y = -3$, $y = -1/2$, $4x - 3 = 10$,  $x = 13/4$

Problem 2.2: (2.3 #29. Introduction to Linear Algebra: Strang) Find the trianÂ­  
gular matrix E that reduces â€œPascalâ€™s matrixâ€ to a smaller Pascal:  

$$
E \left[\begin{matrix} 
1 & 0 &0 & 0 \\
1 & 1 &0 & 0 \\
1 & 2 &1 & 0 \\
1 & 3 &3 & 1 \\
\end{matrix}\right] = 
\left[\begin{matrix} 
1 & 0 &0 & 0 \\
0 & 1 &0 & 0 \\
0 & 1 &1 & 0 \\
0 & 1 &2 & 1 \\
\end{matrix}\right] 
$$
first row <- first row 
second row <- second - first row 
third row <- third row - second row
etc

$$
E = \left[\begin{matrix} 
1 & 0 &0 & 0 \\
-1 & 1 &0 & 0 \\
0 & -1 &1 & 0 \\
0 & 0 &-1 & 1 \\
\end{matrix}\right] $$

Check:

$$
\left[\begin{matrix} 
1 & 0 &0 & 0 \\
-1 & 1 &0 & 0 \\
0 & -1 &1 & 0 \\
0 & 0 &-1 & 1 \\
\end{matrix}\right ]
\left[\begin{matrix} 
1 & 0 &0 & 0 \\
1 & 1 &0 & 0 \\
1 & 2 &1 & 0 \\
1 & 3 &3 & 1 \\
\end{matrix}\right] = 

\left[\begin{matrix} 
1 & 0 &0 & 0 \\
0 & 1 &0 & 0 \\
0 & 1 &1 & 0 \\
0 & 1 &2 & 1 \\
\end{matrix}\right]
$$

Which matrix M (multiplying several Eâ€™s) reduces Pascal all the way  
to I?

$$
E_1 = 
\left[\begin{matrix} 
1 & 0 &0 & 0 \\
-1 & 1 &0 & 0 \\
0 & -1 &1 & 0 \\
0 & 0 &-1 & 1 \\
\end{matrix}\right ]
$$
$$
E_2 = 
\left[\begin{matrix} 
1 & 0 &0 & 0 \\
0 & 1 &0 & 0 \\
0 & -1 &1 & 0 \\
0 & 0 &-1 & 1 \\
\end{matrix}\right ]
$$
$$
E_3 = 
\left[\begin{matrix} 
1 & 0 &0 & 0 \\
0 & 1 &0 & 0 \\
0 & 0 &1 & 0 \\
0 & 0 &-1 & 1 \\
\end{matrix}\right ]
$$
$$
E = E_3E_2 E_1 =  
\left[\begin{matrix} 
1 & 0 &0 & 0 \\
0 & 1 &0 & 0 \\
0 & 0 &1 & 0 \\
0 & 0 &-1 & 1 \\
\end{matrix}\right ]
\left[\begin{matrix} 
1 & 0 &0 & 0 \\
0 & 1 &0 & 0 \\
0 & -1 &1 & 0 \\
0 & 0 &-1 & 1 \\
\end{matrix}\right ]
\left[\begin{matrix} 
1 & 0 &0 & 0 \\
-1 & 1 &0 & 0 \\
0 & -1 &1 & 0 \\
0 & 0 &-1 & 1 \\
\end{matrix}\right ] =
\left[\begin{matrix} 
1 & 0 &0 & 0 \\
0 & 1 &0 & 0 \\
0 & 0 &1 & 0 \\
0 & 0 &-1 & 1 \\
\end{matrix}\right ]
\left[\begin{matrix} 
1 & 0 &0 & 0 \\
-1 & 1 &0 & 0 \\
1 & -2 &1 & 0 \\
0 & 1 &-2 & 1 \\
\end{matrix}\right ] 
$$

$$
E = \left[\begin{matrix} 
1 & 0 &0 & 0 \\
-1 & 1 &0 & 0 \\
1 & -2 &1 & 0 \\
-1 & 3 &-3 & 1 \\
\end{matrix}\right ]
$$


$$EA = 

\left[\begin{matrix} 
1 & 0 &0 & 0 \\
-1 & 1 &0 & 0 \\
1 & -2 &1 & 0 \\
-1 & 3 &-3 & 1 \\
\end{matrix}\right ]
\left[\begin{matrix} 
1 & 0 &0 & 0 \\
1 & 1 &0 & 0 \\
1 & 2 &1 & 0 \\
1 & 3 &3 & 1 \\
\end{matrix}\right] 
= 
\left[\begin{matrix} 
1 & 0 &0 & 0 \\
0 & 1 &0 & 0 \\
0 & 0 &1 & 0 \\
0 & 0 &0 & 1 \\
\end{matrix}\right]


$$


### HW1

#### 1.2

23) ![[Pasted image 20220312113355.png]]

$$\cos \beta = w_1/||w||$$
$$\sin \beta = w_2/||w||$$

$$
\cos \theta = \cos \beta \cos \alpha + \sin \beta \sin \alpha 
$$
$$
\cos \theta = \frac{w_1v_1+w_2v_2}{||w||||v||} = \frac{v \cdot w}{||v|| ||w||}
$$

28) ![[Pasted image 20220312133028.png]]

Let $u$ be $1,0$; $v$ be $-.5,1$; $w$ be $-.5,-1$.

Then $uv = -.5$; $vw = -.75$; $uw = -.5$

29) ![[Pasted image 20220312114206.png]]

Let $x = 1, y = -1, z = 2$. Then $v = (1,-1,2)$ and $w = (2, 1, -1)$. 
Then $v \cdot w = 2 -1 - 2 = -1$. From the below, we know that $\cos \theta$ is $-\frac{1}{2}$. This means the angle is 210 degrees.


The formula returns:
$$ ||v|| = ||w|| = \sqrt{x^2 + y^2 + z^2}$$
$$ \frac{v \cdot w}{||v|| ||w||}  = \frac{xz + yx + zy}{x^2 + y^2 + z^2} $$
$$ (x + y + z)(x + y + z) = x^2  + y^2 + z^2+ 2xy + 2yz + 2xz = 0 $$
$$ xz + yx + zy = -\frac{x^2 + y^2 + z^2}{2}$$
$$ \frac{v \cdot w}{||v|| ||w||} = \frac{-\frac{x^2 + y^2 + z^2}{2}}{x^2 + y^2 + z^2} $$
$$ \frac{v \cdot w}{||v|| ||w||} = - \frac{1}{2}$$

#### 1.3


4) ![[Pasted image 20220312133709.png]]
These vectors are dependent: $w_1 + w_3 - 2w_2 = 0$, meaning that one can be constructed out of linear combinations of the others. This means they all lie in a plane. 

13)  ![[Pasted image 20220312133957.png]]

The $5x5$ centered difference matrix times a vector $b_1 \ldots b_5$ is 

$$\left[ \begin{matrix}
0 & 1 & 0 & 0 &0 \\
-1 &0 & 1 & 0 &0 \\
0 &-1 & 0 & 1 &0 \\
0 & 0 &-1 & 0 &1 \\
0 & 0 & 0 &-1 &0 \\
\end{matrix} \right] \left[ \begin{matrix} b_1 \\ b_2 \\ b_3 \\ b_4 \\ b_5 \end{matrix}\right] = b_1 \left[ \begin{matrix} 0 \\-1 \\ 0 \\ 0 \\ 0\\ \end{matrix}\right] + b_2 \left[ \begin{matrix} 1 \\ 0 \\-1 \\ 0 \\ 0\\ \end{matrix}\right] + b_3 \left[ \begin{matrix} 0 \\ 1 \\ 0 \\-1 \\ 0\\ \end{matrix}\right] + b_4 \left[ \begin{matrix} 0 \\ 0 \\ 1 \\ 0 \\ -1\\ \end{matrix}\right] + b_5 \left[ \begin{matrix} 0 \\ 0 \\ 0 \\ 1 \\ 0\\ \end{matrix}\right]
$$
The following combination gives $0$: $b_1 = b_3 = b_5 = 1$; $b_2 = b_4 = 0$.

#### 2.1

29) ![[Pasted image 20220312135005.png]]

$$u_2 = Au_1 = \left[ \begin{matrix} .8 & .3 \\ .2 & .7 \end{matrix}\right]\left[ \begin{matrix} .8 \\ .2 \end{matrix}\right] = \left[ \begin{matrix} .7 \\ .3 \end{matrix}\right]$$
$$u_3 = Au_2 =  \left[ \begin{matrix} .8 & .3 \\ .2 & .7 \end{matrix}\right]\left[ \begin{matrix} .7 \\ .3 \end{matrix}\right] = \left[ \begin{matrix} .65 \\ .35 \end{matrix}\right]$$

All these matrices add up to 1. 

30) ![[Pasted image 20220312135021.png]]

Steady state is .6, .4

#### 2.2

20) ![[Pasted image 20220312140011.png]]

Linear combination.

We can just add these rows to get an equation: 2x - y = 1

32)![[Pasted image 20220312140208.png]]
a) 0
b) 0

matrix: first row is 1, ... 100; 2, ... 200, and so on

#### 2.3

22) ![[Pasted image 20220312140704.png]]

a) $\sum a_{3j} x_j$
b) $a_{2,1} - a_{1,1}$
c) $a_{2,1} - 2a_{1,1}$
d) $\sum a_{1j} x_j$


29) see practice above
 
#### 2.4

32)

36)

#### 2.5

7)

