---
aliases: 
tags: 
creation date: Thursday, August 11th 2022, 1:10 pm
date updated: Thursday, August 11th 2022, 1:41 pm
---

![[Pasted image 20220811131122.png]]

$$ \lim_{h \to 0} \frac{(a(x+h)^2 + c) - (ax^2 + c)}{h}$$
$$ \lim_{h \to 0} \frac{ax^2+2ahx + ah^2 + c - ax^2 + c}{h}$$
$$ \lim_{h \to 0} \frac{2axh + h^2}{h}$$
Already we can see that $c$ falls out. Factoring gives us $2ax + h$ which approaches $2ax$.


![[Pasted image 20220811131534.png]]

a) $15x^4 + 12x^2 - 14x$
b) $5x + 5^x\ln 5 + 5$
c)$1/3(e^x + x)(e^x + 1)$
d) 
$$\begin{align}
\frac{d}{dx} [x^3 -1]\inv[x^3 + 1] &= (x^3-1)\inv [d/dx (x^3+1)] + [d/dx (x^3 -1)\inv](x^3 + 1) \\
&= 3x^2(x^3-1)\inv -(x^3 -1)^{-2}(3x^2)(x^3 + 1) \\
&= 3x^2\left[\frac{x^3 -1 }{(x^3 - 1)^2} - \frac{x^3 + 1}{(x^3 - 1)^2}\right]\\
&= \frac{-6x^2}{(x^3-1)^2}
\end{align}$$

e) Interpreting this: 

$$\begin{align}
\frac{d}{dx} \ln \left[(x^4 + 1)(x^4 -1)\right]^\frac{1}{2} &= \frac{1}{2}\frac{d}{dx} \left[\ln (x^4 + 1) + \ln(x^4 -1)\right]\\
&= \frac{1}{2}\left[4x^3/(x^4 + 1) + 4x^3/(x^4-1) \right]
\end{align}$$
f) $3x^2e^{4x^2} + 8x^4e^{4x^2}$


![[Pasted image 20220811134301.png]]

a) First derivative is $x^2 -12$, and second is $2x$. 
Increasing where $(x^2
