---
date updated: 2022-04-22 17:04

notetype: "Math Class Note"
cssclass: math-class-note

tags: 
- '#types/classes/math/linalg'
- '#status/ðŸš§'
---
[[18.06 Strang]]

## Practice
### Recitation 8 
We want to solve a non-homogeneous system:

$$
\begin{aligned} 
x -2y -2z &= b_1\\
2x -5y - 4z &= b_2\\
4x -9y-8z &= b_3 \\
\end{aligned}
$$
$$[A \quad b\,] = \begin{bmatrix} 1 & -2 & -2 &|& b_1 \\
2 & -5 & -4 &|& b_2\\
4 & -9 & -8 &|& b_3\\
\end{bmatrix} $$
Worth noting here that this matrix does not have full row rank. So we will have a constraint $2b_1 + b_2 = b_3$. Let's find that by elimination.

$$
\begin{bmatrix} 1 & -2 & -2 &|& b_1 \\
0 & -1 & 0 &|& b_2-2b_1\\
0 & -1 & 0 &|& b_3-4b_1\\
\end{bmatrix} 
$$
$$
\begin{bmatrix} 1 & -2 & -2 &|& b_1 \\
0 & 1 & 0 &|& 2b_1-b_2\\
0 & 0 & 0 &|& b_3- 2b_1 - b_2\\
\end{bmatrix} 
$$
$$
\begin{bmatrix} 1 & 0 & -2 &|& 5b_1 - 2b_2 \\
0 & 1 & 0 &|& 2b_1-b_2\\
0 & 0 & 0 &|& b_3- 2b_1 - b_2\\
\end{bmatrix} 
$$
Here's our constraint. 
Now let's find a particular solution. We can set $z$ to $0$ since it is free. Then let's say $x = 5b_1 - 2b_2$ and $y = 2b_1 - b_2$. We know that works from the above. But a quick confirmation by plugging in to the initial set of equations:

$$
\begin{aligned} 
(5b_1 - 2b_2) -2(2b_1 - b_2) -2(0) &= b_1\\
2(5b_1 - 2b_2) -5(2b_1 - b_2) - 4(0) &= b_2\\
4(5b_1 - 2b_2) -9(2b_1 - b_2)-8(0) &= b_3 \\
\end{aligned}
$$
$$
\begin{aligned} 
5b_1 - 2b_2 -4b_1 +2 b_2&= b_1\\
10b_1 - 4b_2 -10b_1 + 5b_2&= b_2\\
20b_1 - 8b_2 -18b_1 + 9 b_2 &= b_3 \\
\end{aligned}
$$

$$
\begin{aligned} 
b_1&= b_1\\
b_2&= b_2\\
2b_1 + b_2&= b_3 \\
\end{aligned}
$$

Hooray!

Now we can just add the null space of $A$ in - which we know to be dimension $1$ (a line). What are the special solutions to $Ax = 0$? Well, we set the free variables to $1$, one at a time. So $z=1$ gives us $x = 2$. 

(aside) looks like taking 
$$ F = \begin{bmatrix}-2 & 0 \\ 0 & 0 \end{bmatrix}$$
and then stacking $[-F \quad I]'$.

So the solutions are the line:

$$ 
\begin{bmatrix} 
5b_1 - 2 b_2\\
2b_1 - b_2 \\
0\\
\end{bmatrix}
+ c_1
\begin{bmatrix}
2\\0\\1
\end{bmatrix}
$$

### Practice 8


## HW3
